---
draft: true
---
<!-- \sum_{i=1}^{n}{\sum_{j=i+1}^{n}{\(a_i-a_j\)^{2}}}\\
=\frac{1}{2}\times \sum_{i=1}^{n}{\sum_{j=1}^{n}{\(a_i-a_j\)^{2}}}\\
=\frac{1}{2}\times \sum_{i=1}^{n}{\sum_{j=1}^{n}{\(a_i^2+a_j^2-2a_ia_j\)}}\\
=\frac{1}{2}\times \(\sum_{i=1}^{n}{\sum_{j=1}^{n}{a_i^2}}+\sum_{i=1}^{n}{\sum_{j=1}^{n}{a_j^2}}-2\sum_{i=1}^{n}{\sum_{j=1}^{n}{a_ia_j}}\)\\
=\frac{1}{2}\times \(2\sum_{i=1}^{n}{\sum_{j=1}^{n}{a_i^2}}-2\sum_{i=1}^{n}{\sum_{j=1}^{n}{a_ia_j}}\)\\
=\sum_{i=1}^{n}{\sum_{j=1}^{n}{a_i^2}}-\sum_{i=1}^{n}{\sum_{j=1}^{n}{a_ia_j}}\\
=\sum_{i=1}^{n}{a_i^2\sum_{j=1}^{n}{1}}-\sum_{i=1}^{n}{a_i\sum_{j=1}^{n}{a_j}}\\
=n\sum_{i=1}^{n}{a_i^2}-\(\sum_{i=1}^{n}{a_i}\)^2\\
 -->